finish callstate matching f or TaggedNumberedComp

src/TaggedComp.v
@@ -506,87 +506,11 @@ Section Preservation.
 
   Hypothesis TRANSF : compile_cu prog = Some tprog.
 
-  Lemma prog_init_expr :
-    forall expr,
-      In expr (A.initial_env prog) ->
-      exists expr',
-        In expr' (B.initial_env tprog) /\ I_expr expr expr'.
-  Proof.
-    destruct prog. generalize dependent tprog.
-    clear TRANSF.
-    unfold compile_cu.
-    unfold bind_option.
-    induction l; intros.
-    solve [simpl in H; inv H].
-    simpl in IHl.
-    repeat (break_match_hyp; try congruence; [idtac]).
-    repeat (break_inner_match_hyp; try congruence; [idtac]).
-    subst. simpl in H. unfold B.initial_env. inv TRANSF. simpl.
-    simpl in Heqo.
-    unfold seq in *. unfold bind_option in *.
-    unfold fmap in *.
-    repeat (break_match_hyp; try congruence; [idtac]).
-    inv Heqo. inv Heqo2. inv Heqo0.
-    destruct H.
-    * subst. eapply compile_I_expr in H1. simpl.
-      eexists. split. left. reflexivity. eauto.
-    * edestruct IHl; eauto. unfold B.initial_env in *.
-      simpl in *. break_and.
-      exists x. split. right. assumption. assumption.
-  Qed.
-(*  
-  Lemma initial_state_match :
-    forall s,
-      initial_state (A.semantics prog) s ->
-      exists s',
-        initial_state (B.semantics tprog) s' /\ I s s'.
-  Proof.
-    intros. inv H.
-    eapply prog_init_expr in H0.
-    break_exists. break_and.
-    eexists. split. econstructor; eauto.
-    econstructor; eauto. intros.
-    econstructor; eauto.
-  Qed.
- *)
-  Definition match_values (v : A.valtype) (v' : B.valtype) :=
-    v = v'.
-  
-  Lemma match_final_state :
-    forall s s' v,
-      I s s' ->
-      final_state (A.semantics prog) s v ->
-      exists v',
-        final_state (B.semantics tprog) s' v' /\ match_values v v'.
-  Proof.
-    intros. inv H0. inv H.
-    eexists; split.
-    econstructor; eauto.
-    reflexivity.
-  Qed.
-
-  Lemma match_initial_env :
-    Forall2 I_expr (A.initial_env prog) (B.initial_env tprog).
-  Proof.
-    unfold A.initial_env.
-    unfold B.initial_env.
-    unfold compile_cu in *.
-    repeat (break_match_hyp; try congruence). subst.
-    simpl.
-    eapply compile_list_I_expr; eauto.
-    unfold bind_option in *. break_match_hyp; try congruence. inv TRANSF. reflexivity.
-  Qed.
-
   Theorem fsim :
     forward_simulation (Lifted.semantics prog) (Tagged.semantics tprog).
   Proof.
-    eapply forward_simulation_step.
+    (* This whole proof needs to be redone to connect up to Untyped8 instead of Lifted. *)
     admit.
-    eapply match_final_state; eauto.
-    intros.
-    unfold Lifted.semantics in *. simpl in *.
-    eapply I_sim; eauto.
-    eapply match_initial_env.
   Admitted.
 
 End Preservation.
